Core/Logic.v
@@ -16,52 +16,53 @@ End OBJECT.
 Module Predicates(O : OBJECT).
   Import O.
 
-  Definition Prec := @InterState E VE -> Trace (ThreadEvent F) -> Prop.
-
-  Definition Relt :=
-    @InterState E VE -> Trace (ThreadEvent F) ->
-    @InterState E VE -> Trace (ThreadEvent F) ->
+  Definition Prec :=
+    @InterState E F VE ->
+    Trace (ThreadEvent F) ->
     Prop.
 
-  Definition Post A := A -> Relt.
+  Definition Relt :=
+    @InterState E F VE -> Trace (ThreadEvent F) ->
+    @InterState E F VE -> Trace (ThreadEvent F) ->
+    Prop.
 
-  Definition Prec_to_Relt (P : Prec) : Relt :=
+  Definition PrecToRelt (P : Prec) : Relt :=
     fun s ρ t σ => s = t /\ ρ = σ /\ P t σ.
-  Coercion Prec_to_Relt : Prec >-> Relt.
-  Definition Relt_to_Prec (R : Relt) : Prec :=
+  Coercion PrecToRelt : Prec >-> Relt.
+  Definition ReltToPrec (R : Relt) : Prec :=
     fun t σ => exists s ρ, R s ρ t σ.
-  Coercion Relt_to_Prec : Relt >-> Prec.
+  Coercion ReltToPrec : Relt >-> Prec.
 
-  Definition Relt_compose (R G : Relt) : Relt :=
+  Definition ReltCompose (R G : Relt) : Relt :=
     fun s ρ r τ => exists t σ, R s ρ t σ /\ G t σ r τ.
-  Notation "R ; G" := (Relt_compose R G) (right associativity, at level 39).
+  Notation "R ; G" := (ReltCompose R G) (right associativity, at level 39).
 
   Class HasImpl A :=
     impl : A -> A -> A.
-  Notation "P ==> Q" := (impl P Q) (right associativity, at level 35).
+  Notation "P ==> Q" := (impl P Q) (right associativity, at level 41).
   
-  Global Instance impl_Prec : HasImpl Prec :=
+  Global Instance implPrec : HasImpl Prec :=
     fun P Q s ρ => P s ρ -> Q s ρ.
   
-  Global Instance impl_Relt : HasImpl Relt :=
+  Global Instance implRelt : HasImpl Relt :=
     fun P Q s ρ t σ => P s ρ t σ -> Q s ρ t σ.
   
   Class HasStable A :=
     Stable : Relt -> A -> Prop.
   
-  Global Instance stable_Relt : HasStable Relt :=
+  Global Instance stableRelt : HasStable Relt :=
     fun R Q => forall s ρ t σ, (R; Q ==> Q) s ρ t σ /\ (Q; R ==> Q) s ρ t σ.
   
-  Global Instance stable_Prec : HasStable Prec :=
+  Global Instance stablePrec : HasStable Prec :=
     fun R P => forall s ρ, ((fun t σ => exists s ρ, P s ρ /\ R s ρ t σ) ==> P) s ρ.
 
   Class HasAll A :=
     All : A -> Prop.
   
-  Global Instance all_Relt : HasAll Relt :=
+  Global Instance allRelt : HasAll Relt :=
     fun R => forall s ρ t σ, R s ρ t σ.
   
-  Global Instance all_Prec : HasAll Prec :=
+  Global Instance allPrec : HasAll Prec :=
     fun P => forall s ρ, P s ρ.
   
   Definition id : Relt :=
@@ -71,6 +72,56 @@ Module Predicates(O : OBJECT).
     fun _ _ => True.
   Definition rtop : Relt :=
     fun _ _ _ _ => True.
+
+  Lemma stableRight {R Q : Relt} : Stable R Q -> All ((Q; R) ==> Q).
+  unfold Stable, stableRelt, All, allRelt.
+  intros.
+  specialize (H s ρ t σ).
+  destruct H.
+  easy.
+  Qed.
+
+  Lemma stableLeft {R Q : Relt} : Stable R Q -> All ((R; Q) ==> Q).
+  unfold Stable, stableRelt, All, allRelt.
+  intros.
+  specialize (H s ρ t σ).
+  destruct H.
+  easy.
+  Qed.
+
+  Lemma compStable {R Q S : Relt} :
+    Stable R Q ->
+    Stable R S ->
+    Stable R (Q; S).
+  intros.
+  unfold Stable, stableRelt, impl, implRelt.
+  intros.
+  split.
+  intros.
+  do 3 destruct H1.
+  do 3 destruct H2.
+  do 2 eexists.
+  split.
+  eapply stableLeft.
+  easy.
+  do 2 eexists.
+  split.
+  exact H1.
+  exact H2.
+  easy.
+  intros.
+  do 6 destruct H1.
+  do 2 eexists.
+  split.
+  exact H1.
+  eapply stableRight.
+  easy.
+  do 2 eexists.
+  split.
+  exact H3.
+  easy.
+  Qed.
+
 End Predicates.
 
 Module Logic(O : OBJECT).
@@ -82,23 +133,27 @@ Module Logic(O : OBJECT).
     (at level 20).
 
   Definition Commit i (impl : Impl E F)
-    (G : Relt)
+    (R G : Relt)
     (P : Prec)
     (ev : @Event E)
     (Q : Relt) :=
     forall s ρ t,
-    LinToVF ρ ->
+    LinToSpec ρ VF ->
     P s ρ ->
-      InterStep (impl:=impl) i s (i, liftUEv ev) t /\
+    InterStep (impl:=impl) i s (i, liftUEv ev) t ->
       exists σ,
         Q s ρ t σ /\
         G s ρ t σ /\
         ρ --> σ.
- 
-  Definition VerifyPrim i (impl : Impl E F) (R G : Relt) (P : Prec) (ev : @Event E) (Q : Relt) :=
+  
+  Definition VerifyPrim i (impl : Impl E F)
+    (R G : Relt)
+    (P : Prec)
+    (ev : @Event E)
+    (Q : Relt) :=
     Stable R P /\
     Stable R Q /\
-    Commit i impl G P ev Q.
+    Commit i impl R G P ev Q.
 
   CoInductive VerifyProg i (impl : Impl E F) : Relt -> Relt -> forall (A: Type), Prec -> Prog E A -> Relt -> Prop :=
   | SafeReturn A v :
@@ -106,23 +161,31 @@ Module Logic(O : OBJECT).
   | SafeBind A B R G P QI QR S (m : E A) (k : A -> Prog E B) :
       VerifyPrim i impl R G P (CallEv m) QI ->
       (forall v,
-        VerifyPrim i impl R G (P; QI) (RetEv v) QR /\
+        VerifyPrim i impl R G (P; QI) (RetEv m v) QR /\
         VerifyProg i impl R G B (P; QI; QR) (k v) S) ->
       VerifyProg i impl R G B P (Bind m k) (QI; QR; S)
   | SafeNoOp A R G P C Q :
       VerifyProg i impl R G A P C Q ->
       VerifyProg i impl R G A P (NoOp C) Q
-  | SafeWeaken A C R R' G G' P P' Q Q' :
-      Stable R' P' ->
-      Stable R' Q' ->
-      All (P' ==> P) ->
-      All (R' ==> R) ->
-      All (G ==> G') ->
-      All (Q ==> Q') ->
-      VerifyProg i impl R G A P C Q ->
-      VerifyProg i impl R' G' A P' C Q'
   .
   Arguments VerifyProg i impl R G {A} P C Q.
+
+  Lemma SafeWeaken {i impl A} {C : Prog E A} R R' G G' P P' Q Q' :
+    VerifyProg i impl R G P C Q ->
+    Stable R' P' ->
+    Stable R' Q' ->
+    All (P' ==> P) ->
+    All (R' ==> R) ->
+    All (G ==> G') ->
+    All (Q ==> Q') ->
+    VerifyProg i impl R' G' P' C Q'.
+  Admitted.
+
+  Lemma SafeWeakenPost {i impl A} {C : Prog E A} R G P Q Q' :
+    VerifyProg i impl R G P C Q ->
+    Stable R Q' ->
+    VerifyProg i impl R G P C Q'.
+  Admitted.
 
   Definition TIdle (i : ThreadName) : Prec :=
     fun s ρ =>
@@ -134,40 +197,47 @@ Module Logic(O : OBJECT).
       TIdle i s ρ /\
       σ = app ρ (cons (i, CallEv m) nil) /\
       InterStep (impl:=impl) i s (i, OCallEv m) t.
+  
+  Definition InvokeAny impl i : Relt :=
+    fun s ρ t σ => exists Ret (m : F Ret), Invoke impl i Ret m s ρ t σ.
 
-  Definition Returned (i : ThreadName) (Ret : Type) : Relt :=
+  Definition Returned (i : ThreadName) {Ret} (m : F Ret) : Relt :=
     fun s ρ t σ =>
       s = t /\ ρ = σ /\
       exists (v : Ret), 
-        fst t i = Cont (Return v) /\
+        fst t i = Cont m (Return v) /\
         exists r,
-          projAgent i σ = app r (cons (i, RetEv v) nil).
+          projAgent i σ = app r (cons (i, RetEv m v) nil).
 
-  Definition Return (impl : Impl E F) (i : ThreadName) (Ret : Type) : Relt :=
+  Definition Return (impl : Impl E F) (i : ThreadName) {Ret} (m : F Ret) : Relt :=
     fun s ρ t σ =>
       fst t i = Idle /\
       σ = ρ /\
       exists (v : Ret) r,
-        projAgent i σ = app r (cons (i, RetEv v) nil) /\
-        InterStep (impl:=impl) i s (i, ORetEv v) t.
+        projAgent i σ = app r (cons (i, RetEv m v) nil) /\
+        InterStep (impl:=impl) i s (i, ORetEv m v) t.
+
+  Definition ReturnAny impl i : Relt :=
+    fun s ρ t σ => exists Ret (m : F Ret), Return impl i m s ρ t σ.
 
   Definition VerifyImpl
-    (R G : Relt)
-    (P : forall Ret, F Ret -> Prec)
+    (R G : ThreadName -> Relt)
+    (P : ThreadName -> forall Ret, F Ret -> Prec)
     (impl : Impl E F)
-    (Q : forall Ret, F Ret -> Relt) : Prop :=
-    All (G ==> R) /\
+    (Q : ThreadName -> forall Ret, F Ret -> Relt) : Prop :=
     (forall i Ret (m : F Ret),
-      P Ret m (allIdle, VE.(Init)) nil /\
-      All (P Ret m ==> TIdle i) /\
-      Stable R (P Ret m) /\
-      Stable R (Q Ret m) /\
-      VerifyProg i impl R G
-        (P Ret m; Invoke impl i Ret m)
+      VerifyProg i impl (R i) (G i)
+        (P i Ret m; Invoke impl i Ret m)
         (impl Ret m)
-        (Q Ret m; Returned i Ret)) /\
+        (Q i Ret m; Returned i m)) /\
+    (forall i Ret (m : F Ret),
+      P i Ret m (allIdle, VE.(Init)) nil /\
+      All (P i Ret m ==> TIdle i) /\
+      Stable (R i) (P i Ret m) /\
+      Stable (R i) (Q i Ret m)) /\
+    (forall i, All (G i ==> R i)) /\
     (forall i Ret1 (m1 : F Ret1) Ret2 (m2 : F Ret2),
-      All (P Ret1 m1; Invoke impl i Ret1 m1; Q Ret1 m1; Returned i Ret1; Return impl i Ret1 ==> P Ret2 m2)).
+      All (P i Ret1 m1; Invoke impl i Ret1 m1; Q i Ret1 m1; Returned i m1; Return impl i m1 ==> P i Ret2 m2)).
   
   (* Theorem soundness (lay : Layer E F) :
     (exists R G P Q, VerifyImpl R G P lay.(LImpl) Q) ->
