Examples/AtomicCounter.v
@@ -1,35 +1,249 @@
 From LHL.Core Require Import
-    Program
-    Specs.
+  Program
+  Specs
+  Logic
+  Tensor
+  Traces
+  Linearizability.
 
 From LHL.Examples Require Import
-    RacyCounter
-    CounterSpecs
-    Lock.
+  RacyCounter
+  CounterSpecs
+  Lock.
+
+From Coq Require Import
+  Program.Equality
+  Lists.List
+  Relations.Relation_Operators.
 
 Definition atomicCounterSpec : Spec CounterSig := {|
-    State := AtomicCounterState;
-    Step := AtomicCounterStep;
-    Init := CounterIdle 0
+  State := AtomicCounterState;
+  Step := AtomicCounterStep;
+  Init := CounterIdle 0
 |}.
 
 Definition Underlay := LockSig |+| CounterSig.
 
 Definition inc : Prog Underlay unit :=
-    _ <- InL Acq;
-    _ <- InR Inc;
-    _ <- InL Rel;
-    Return tt.
+  _ <- inl Acq;
+  _ <- inr Inc;
+  _ <- inl Rel;
+  Return tt.
 
 Definition get : Prog Underlay nat :=
-    _ <- InL Acq;
-    n <- InR Get;
-    _ <- InL Rel;
-    Return n.
+  _ <- inl Acq;
+  n <- inr Get;
+  _ <- inl Rel;
+  Return n.
 
 Definition atomicCounterImpl : Impl (LockSig |+| CounterSig) CounterSig :=
-    fun _ m => match m with
-    | Inc => inc
-    | Get => get
+  fun _ m => match m with
+  | Inc => inc
+  | Get => get
+  end.
+
+Module AtomicCounterObj <: OBJECT.
+  Definition E := Underlay.
+  Definition F := CounterSig.
+  Definition VE := tensorSpec lockSpec racyCounterSpec.
+  Definition VF := atomicCounterSpec.
+End AtomicCounterObj.
+
+Module Logic := Logic(AtomicCounterObj).
+Import AtomicCounterObj.
+Import Logic.
+Import Ps.
+
+Definition countState (s : @InterState E F VE) : RacyCounterState :=
+  snd (snd s).
+
+Definition lockState (s : @InterState E F VE) : LockState :=
+  fst (snd s).
+
+Definition int : Relt :=
+  fun s ρ t σ =>
+    exists i,
+    (exists A (m : F A),
+      InterStep (impl:=atomicCounterImpl) i s (i, OCallEv m) t) \/
+    (exists A (m : F A) v,
+      InterStep (impl:=atomicCounterImpl) i s (i, ORetEv m v) t).
+
+Definition rely : ThreadName -> Relt :=
+  fun i s ρ t σ =>
+    int s ρ t σ \/
+    (lockState t = LockOwned i ->
+      countState s = countState t /\
+      lin VF ρ = lin VF σ).
+
+Definition guar : ThreadName -> Relt :=
+  fun i s ρ t σ =>
+    int s ρ t σ \/
+    (lockState t <> LockOwned i ->
+      countState s = countState t /\
+      lin VF ρ = lin VF σ).
+
+Definition precs : ThreadName -> forall Ret, CounterSig Ret -> Prec :=
+  fun i Ret m s ρ =>
+    TIdle i s ρ /\
+    countState s <> CounterUB /\
+    lockState s <> LockOwned i.
+
+Definition posts : ThreadName -> forall Ret, CounterSig Ret -> Relt :=
+  fun i Ret m s ρ t σ =>
+    lockState s <> LockOwned i /\
+    exists n,
+    countState s = CounterDSt (CounterIdle n) /\
+    match m with
+    | Get => True
+    | Inc => countState t = CounterDSt (CounterIdle (S n))
     end.
 
+Ltac psimpl :=
+repeat repeat match goal with
+| [ H : ReltCompose ?P ?Q ?s ?ρ ?t ?σ |- ?G] => destruct H
+| [ H : ?P /\ ?Q |- ?G ] => destruct H
+| [ H : exists x, ?P |- ?G ] => destruct H
+| [ H : ReltToPrec ?R ?s ?ρ |- ?G ] => destruct H
+| [ H : PrecToRelt ?P ?s ?ρ ?t ?σ |- ?G ] => destruct H
+| [ H : Invoke ?impl ?i ?A ?l ?s ?ρ ?t ?σ |- ?G ] => destruct H
+end;
+repeat match goal with
+| [ H : InterStep ?i ?st ?ev ?st' |- ?G ] => dependent destruction H
+| [ H : Step ?impl ?st ?ev ?st' |- ?G ] => idtac ev; simpl in H; dependent destruction H
+end;
+simpl in *;
+subst.
+
+Ltac commit :=
+unfold Commit;
+intros;
+repeat psimpl.
+
+Lemma new_poss_refl : forall (ρ : Trace (ThreadEvent F)), ρ --> ρ.
+intros.
+exists nil.
+split.
+constructor.
+rewrite app_nil_r.
+exists nil, nil.
+split.
+constructor.
+split.
+constructor.
+apply rt_refl.
+Qed.
+
+Theorem atomicCounterCorrect :
+    VerifyImpl rely guar precs atomicCounterImpl posts.
+unfold VerifyImpl.
+split.
+intros.
+dependent destruction m; simpl.
+unfold inc.
+eapply SafeWeakenPost.
+eapply SafeBind with
+  (QI:= fun s ρ t σ =>
+    lockState t = LockAcqRunning i /\
+    σ = ρ)
+  (QR:= fun s ρ t σ =>
+    lockState t = LockOwned i /\
+    σ = app ρ (cons (i, RetEv Inc tt) nil)).
+{
+  unfold VerifyPrim.
+  split.
+  {
+    unfold Stable, stablePrec, impl, implPrec.
+    intros.
+    do 10 destruct H.
+  }
+  split.
+  admit.
+  commit.
+  dependent destruction H7.
+  destruct st, st'.
+  simpl in *.
+  subst.
+  eexists.
+  split.
+  easy.
+  unfold guar.
+  split.
+  right.
+  unfold lockState.
+  simpl.
+  intros.
+  easy.
+  apply new_poss_refl.
+}
+intros.
+split.
+{
+  unfold VerifyPrim.
+  split.
+  admit.
+  split.
+  admit.
+  commit.
+  dependent destruction H6.
+  destruct st, st'.
+  simpl in *.
+  subst.
+  eexists.
+  split.
+  easy.
+  unfold guar.
+  split.
+  right.
+  unfold lockState.
+  simpl.
+  intros.
+  easy.
+  exists nil.
+  split.
+  constructor.
+  exists nil, (cons (i, RetEv Inc tt) nil).
+  split.
+  constructor.
+  constructor.
+  constructor.
+  constructor.
+  do 2 rewrite app_nil_r.
+  apply rt_refl.
+}
+eapply SafeBind with
+  (QI:= fun s ρ t σ =>
+    lockState t = LockOwned i /\
+    σ = ρ /\
+    exists n,
+    countState t = CounterDSt (CounterIncRunning n i))
+  (QR:= fun s ρ t σ =>
+    lockState t = LockOwned i /\
+    σ = ρ /\
+    exists n,
+    countState s = CounterDSt (CounterIncRunning n i) /\
+    countState t = CounterDSt (CounterIdle (S n))).
+{
+  unfold VerifyPrim.
+  split.
+  admit.
+  split.
+  admit.
+  commit.
+  
+}
+intros.
+split.
+admit.
+eapply SafeBind with
+  (QI:= fun s ρ t σ =>
+    lockState t = LockRelRunning i /\
+    σ = ρ)
+  (QR:= fun s ρ t σ =>
+    lockState t = LockUnowned /\
+    σ = ρ).
+admit.
+intros.
+split.
+admit.
+eapply SafeWeaken.
+apply SafeReturn.
